\section{Derivation}
\label{sec:derivation}

Let $E_2 = \sum_{p} E_2^p$ where

\begin{equation}
  E_2^p = -\frac{1}{2}\sum_{q=1}^N \sum_{k \in H_c} (a_{H_{c_k}}^p - a_{H_{c_k}}^q)^2
\end{equation}

The gradient of the error $E_2^p$ with respect to $w_{ji}$ is given by

\begin{equation}
  \frac{\partial E_2^p}{\partial w_{ji}} = \sum_{k \in H_c} \frac{\partial E_2^p}{\partial a_{H_{c_k}}^p} \frac{\partial a_{H_{c_k}}^p}{\partial w_{ji}} + \frac{\partial E_2^p}{\partial a_{H_{c_k}}^q} \frac{\partial a_{H_{c_k}}^q}{\partial w_{ji}}
\end{equation}

Because $\partial a_{H_{c_k}}^p = \partial a_{H_{c_k}}^q = 0$ when $k \neq j$,
we can simplify this to get

\begin{align}
  \frac{\partial E_2^p}{\partial w_{ji}} = \frac{\partial E_2^p}{\partial a_{H_{c_j}}^p} \frac{\partial a_{H_{c_j}}^p}{\partial w_{ji}} + \frac{\partial E_2^p}{\partial a_{H_{c_j}}^q} \frac{\partial a_{H_{c_j}}^q}{\partial w_{ji}} \nonumber \\
  = -\frac{1}{2} \sum_{q=1}^N \sum_{k \in H_c} \frac{\partial(a_{H_{c_k}}^p - a_{H_{c_k}}^q)^2}{\partial a_{h_{c_j}}^p} \frac{\partial a_{H_{c_j}}^p}{\partial w_{ji}} \nonumber \\
  + -\frac{1}{2} \sum_{q=1}^N \sum_{k \in H_c} \frac{\partial(a_{H_{c_k}}^p - a_{H_{c_k}}^q)^2}{\partial a_{h_{c_j}}^q} \frac{\partial a_{H_{c_j}}^q}{\partial w_{ji}} \nonumber \\
  = - \sum_{q=1}^N \sum_{k \in H_c} (a_{H_{c_k}}^p-a_{H_{c_k}}^q)(\frac{\partial a_{H_{c_k}}^p}{\partial a_{H_{c_j}}^p}-\frac{\partial a_{H_{c_k}}^q}{\partial a_{H_{c_j}}^p})\frac{\partial a_{H_{c_j}}^p}{\partial w_{ji}} \nonumber \\
  + - \sum_{q=1}^N \sum_{k \in H_c} (a_{H_{c_k}}^p-a_{H_{c_k}}^q)(\frac{\partial a_{H_{c_k}}^p}{\partial a_{H_{c_j}}^q}-\frac{\partial a_{H_{c_k}}^q}{\partial a_{H_{c_j}}^q})\frac{\partial a_{H_{c_j}}^q}{\partial w_{ji}} 
\end{align}

When $k \neq j$, our gradient becomes $0$ as neither $a_{h_{c_k}}^p$ nor $a_{h_{c_k}}^q$
have $w_{ji}$ components so we get

\begin{align}
  \frac{\partial E_2^p}{\partial w_{ji}} = - \sum_{q=1}^N (a_{H_{c_j}}^p-a_{H_{c_j}}^q)(\frac{\partial a_{H_{c_j}}^p}{\partial a_{H_{c_j}}^p}-\frac{\partial a_{H_{c_j}}^q}{\partial a_{H_{c_j}}^p})\frac{\partial a_{H_{c_j}}^p}{\partial w_{ji}} \nonumber \\
  + - \sum_{q=1}^N (a_{H_{c_j}}^p-a_{H_{c_j}}^q)(\frac{\partial a_{H_{c_j}}^p}{\partial a_{H_{c_j}}^q}-\frac{\partial a_{H_{c_j}}^q}{\partial a_{H_{c_j}}^q})\frac{\partial a_{H_{c_j}}^q}{\partial w_{ji}} \nonumber \\
  = \frac{\partial E_2^p}{\partial w_{ji}} = - \sum_{q=1}^N (a_{H_{c_j}}^p-a_{H_{c_j}}^q)(1-\frac{\partial a_{H_{c_j}}^q}{\partial a_{H_{c_j}}^p})\frac{\partial a_{H_{c_j}}^p}{\partial w_{ji}} \label{eq:part_p}\\
  + - \sum_{q=1}^N (a_{H_{c_j}}^p-a_{H_{c_j}}^q)(\frac{\partial a_{H_{c_j}}^p}{\partial a_{H_{c_j}}^q}-1)\frac{\partial a_{H_{c_j}}^q}{\partial w_{ji}} \label{eq:part_q}
\end{align}

%\newpage

We will first consider (\ref{eq:part_p}). For $p = q$, we get a
gradient of $0$ due to the subtraction of the acitavtions
and for $p \neq q$ we get $\partial a_{H_{c_j}}^q / a_{H_{c_j}}^p = 0$ so
we can simplify

\begin{align}
  (\ref{eq:part_p}) = - \sum_{q=1, q \neq p}^N (a_{H_{c_j}}^p-a_{H_{c_j}}^q)\frac{\partial a_{H_{c_j}}^p}{\partial w_{ji}} \nonumber \\
  = -((N-1)a_{H_{c_j}}^p - \sum_{q=1, q \neq p}^N a_{H_{c_j}}^q)\frac{\partial a_{H_{c_j}}^p}{\partial w_{ji}} \nonumber \\
  = -(N a_{H_{c_j}}^p - \sum_{q=1}^N a_{H_{c_j}}^q) \frac{\partial a_{H_{c_j}}^p}{\partial w_{ji}} \nonumber \\
  = -N(a_{H_{c_j}}^p-\overline{a_{H_{c_j}}}) a_{H_{c_j}}^p(1-a_{H_{c_j}}^p) a_{H_{c-1_i}}^p
\label{eq:part_p_simplify}
\end{align}

where $N$ is the number of training patterns and $\overline{a_{H_{c_j}}}$ is the
average activation of the $j^{th}$ hidden unit over all input samples. 

We now consider (\ref{eq:part_q}). Again, for $p=q$ our gradient is $0$.
For $p \neq q$ we get  $\partial a_{H_{c_j}}^p / a_{H_{c_j}}^q = 0$ so we can simplify

\begin{align} \label{eq:part_q_simplify}
  (\ref{eq:part_q}) = \sum_{q=1, q \neq p}^N (a_{H_{c_j}}^p-a_{H_{c_j}}^q)\frac{\partial a_{H_{c_j}}^q}{\partial w_{ji}} \nonumber \\
  = \sum_{q=1, q \neq p}^N (a_{H_{c_j}}^p-a_{H_{c_j}}^q) a_{H_{c_j}}^q(1-a_{H_{c_j}}^q) a_{H_{c-1_i}}^q 
\end{align}

We can now combine (\ref{eq:part_p_simplify}) and (\ref{eq:part_q_simplify}) to get

\begin{align}
  \frac{\partial E_2^p}{\partial w_{ji}} = (\sum_{q=1, q \neq p}^N (a_{H_{c_j}}^p-a_{H_{c_j}}^q) a_{H_{c_j}}^q(1-a_{H_{c_j}}^q) a_{H_{c-1_i}}^q) \nonumber \\
  - N(a_{H_{c_j}}^p-\overline{a_{H_{c_j}}}) a_{H_{c_j}}^p(1-a_{H_{c_j}}^p) a_{H_{c-1_i}}^p
\end{align}



%% Using similar math as show in (\ref{eq:part_p_simplify}), we simplify this to

%% \begin{equation} \label{eq:part_q_simplify1}
%%   (\ref{eq:part_q}) = N(a_{H_{c_j}}^p-\overline{a_{H_{c_j}}}) \
%% \end{equation} 

%% Finally, combining (\ref{eq:part_p_simplify}) and (\ref{eq:part_q_simplify}) we get

%% \begin{equation}
%%   \frac{\partial E_2^p}{\partial w_{ji}} = N(a_{H_{c_j}}^p-\overline{a_{H_{c_j}}})(a_{H_{c_j}}^q(1-a_{H_{c_j}}^q) a_{H_{c-1_i}}^q - a_{H_{c_j}}^p(1-a_{H_{c_j}}^p) a_{H_{c-1_i}}^p)
%% \end{equation}
